examples/map/MapIAproof.v
@@ -1,6 +1,6 @@
 Require Import CRIS.
 
-Require Import MapHeader MapASpec MapMSpec MapI ModSim MapIMproof MapMAproof MemA.
+Require Import MapHeader MapA MapM MapI ModSim MapIMproof MapMAproof MemA.
 
 Module MapIA. Section MapIA.
   Context `{!invG α Σ Γ, !subHG Γ Σ, !sinvG Σ Γ α β τ, !MapAGΓ Γ, !MapMGΓ Γ, !memGΓ Γ}.
@@ -8,8 +8,8 @@ Module MapIA. Section MapIA.
   Theorem correct gi (StbMap StbMem : Sk.t → string → option fspec)
       (MapInStbMap : ∀ sk, stb_incl MapAS.Stb (StbMap sk)) :
     ctx_refines
-      ((MapAS.t gi StbMap)  ★ (MemA.t gi StbMem), MapAS.InitCond ∗∗ MapMS.InitCond)
-      ((MapI.t)             ★ (MemA.t gi StbMem), const(emp%I)).
+      ((MapA.t gi StbMap)  ★ (MemA.t gi StbMem), MapA.InitCond ∗∗ MapM.InitCond)
+      ((MapI.t)            ★ (MemA.t gi StbMem), const(emp%I)).
   Proof.
     etrans; cycle 1.
     { eapply main_adequacy. eapply MapIM.sim.
@@ -18,7 +18,7 @@ Module MapIA. Section MapIA.
     }
     etrans; cycle 1.
     { eapply ctxr_frameR.
-      rewrite -(hmod_addc_empty_l _ MapMS.InitCond).
+      rewrite -(hmod_addc_empty_l _ MapM.InitCond).
       eapply ctxr_cond_frameR, main_adequacy, MapMA.sim; eauto.
       intros sk; split; try refl.
       rewrite /MapMS.Stb; unseal CRIS; prove_nodup.
